Launchbury/Flag.thy
@@ -1,0 +1,16 @@
+theory Flag
+imports Main "Nominal2"
+begin
+
+datatype Flag = FlagSet ("\<surd>") | FlagNotSet ("\<times>")
+
+instantiation  Flag :: pure
+begin
+  definition "p \<bullet> (v::Flag) = v"
+instance
+  apply default
+  apply (auto simp add: permute_Flag_def)
+  done
+end
+
+end
